Extensions/Sound/StableSound.v
@@ -161,7 +161,7 @@ Require Import Logic.PropositionalLogic.Semantics.Kripke.
 Require Import Logic.ModalLogic.Semantics.Flat.
 Require Import Logic.SeparationLogic.Semantics.FlatSemantics.
 
-Lemma sound_impp_stable {L: Language} {nL: NormalLanguage L} {pL: PropositionalLanguage L} {MD: Model} {kMD: KripkeModel MD} {M: Kmodel} {R1: KI.Relation (Kworlds M)} {R2: SS.Relation (Kworlds M)} {R1_bis: Bisimulation SS.Krelation KI.Krelation} {SM: Semantics L MD} {kiSM: KripkeIntuitionisticSemantics L MD M SM} {stableSM: SemanticStable L MD M SM}:
+Lemma sound_impp_stable {L: Language} {nL: NormalLanguage L} {pL: PropositionalLanguage L} {MD: Model} {kMD: KripkeModel MD} {M: Kmodel} {R1: KI.Relation (Kworlds M)} {R2: SS.Relation (Kworlds M)} {R1_bis: Bisimulation SS.Krelation KI.Krelation} {SM: Semantics L MD} {kiSM: KripkeIntuitionisticSemantics L MD M SM} {kpSM: KripkePropositionalSemantics L MD M SM} {stableSM: SemanticStable L MD M SM}:
   forall x y: expr,
     semantic_stable x -> semantic_stable y -> semantic_stable (x --> y).
 Proof.
@@ -191,7 +191,7 @@ Proof.
     tauto.
 Qed.
 
-Lemma sound_andp_stable {L: Language} {nL: NormalLanguage L} {pL: PropositionalLanguage L} {MD: Model} {kMD: KripkeModel MD} {M: Kmodel} {R1: KI.Relation (Kworlds M)} {R2: SS.Relation (Kworlds M)} {SM: Semantics L MD} {kiSM: KripkeIntuitionisticSemantics L MD M SM} {stableSM: SemanticStable L MD M SM}:
+Lemma sound_andp_stable {L: Language} {nL: NormalLanguage L} {pL: PropositionalLanguage L} {MD: Model} {kMD: KripkeModel MD} {M: Kmodel} {R1: KI.Relation (Kworlds M)} {R2: SS.Relation (Kworlds M)} {SM: Semantics L MD} {kiSM: KripkeIntuitionisticSemantics L MD M SM} {kpSM: KripkePropositionalSemantics L MD M SM} {stableSM: SemanticStable L MD M SM}:
   forall x y: expr,
     semantic_stable x -> semantic_stable y -> semantic_stable (x && y).
 Proof.
@@ -206,7 +206,7 @@ Proof.
   tauto.
 Qed.
 
-Lemma sound_orp_stable {L: Language} {nL: NormalLanguage L} {pL: PropositionalLanguage L} {MD: Model} {kMD: KripkeModel MD} {M: Kmodel} {R1: KI.Relation (Kworlds M)} {R2: SS.Relation (Kworlds M)} {SM: Semantics L MD} {kiSM: KripkeIntuitionisticSemantics L MD M SM} {stableSM: SemanticStable L MD M SM}:
+Lemma sound_orp_stable {L: Language} {nL: NormalLanguage L} {pL: PropositionalLanguage L} {MD: Model} {kMD: KripkeModel MD} {M: Kmodel} {R1: KI.Relation (Kworlds M)} {R2: SS.Relation (Kworlds M)} {SM: Semantics L MD} {kiSM: KripkeIntuitionisticSemantics L MD M SM} {kpSM: KripkePropositionalSemantics L MD M SM} {stableSM: SemanticStable L MD M SM}:
   forall x y: expr,
     semantic_stable x -> semantic_stable y -> semantic_stable (x || y).
 Proof.
@@ -221,7 +221,7 @@ Proof.
   tauto.
 Qed.
 
-Lemma sound_falsep_stable {L: Language} {nL: NormalLanguage L} {pL: PropositionalLanguage L} {MD: Model} {kMD: KripkeModel MD} {M: Kmodel} {R1: KI.Relation (Kworlds M)} {R2: SS.Relation (Kworlds M)} {SM: Semantics L MD} {kiSM: KripkeIntuitionisticSemantics L MD M SM} {stableSM: SemanticStable L MD M SM}:
+Lemma sound_falsep_stable {L: Language} {nL: NormalLanguage L} {pL: PropositionalLanguage L} {MD: Model} {kMD: KripkeModel MD} {M: Kmodel} {R1: KI.Relation (Kworlds M)} {R2: SS.Relation (Kworlds M)} {SM: Semantics L MD} {kiSM: KripkeIntuitionisticSemantics L MD M SM} {kpSM: KripkePropositionalSemantics L MD M SM} {stableSM: SemanticStable L MD M SM}:
   semantic_stable falsep.
 Proof.
   intros.
@@ -232,7 +232,7 @@ Proof.
   reflexivity.
 Qed.
 
-Lemma sound_stable_proper_iffp {L: Language} {nL: NormalLanguage L} {pL: PropositionalLanguage L} {MD: Model} {kMD: KripkeModel MD} {M: Kmodel} {R1: KI.Relation (Kworlds M)} {po_R: PreOrder KI.Krelation} {R2: SS.Relation (Kworlds M)} {SM: Semantics L MD} {kiSM: KripkeIntuitionisticSemantics L MD M SM} {stableSM: SemanticStable L MD M SM}:
+Lemma sound_stable_proper_iffp {L: Language} {nL: NormalLanguage L} {pL: PropositionalLanguage L} {MD: Model} {kMD: KripkeModel MD} {M: Kmodel} {R1: KI.Relation (Kworlds M)} {po_R: PreOrder KI.Krelation} {R2: SS.Relation (Kworlds M)} {SM: Semantics L MD} {kiSM: KripkeIntuitionisticSemantics L MD M SM} {kpSM: KripkePropositionalSemantics L MD M SM} {stableSM: SemanticStable L MD M SM}:
   forall x y,
     (forall m, KRIPKE: M, m |= x <--> y) ->
     (semantic_stable x <-> semantic_stable y).
@@ -286,7 +286,7 @@ Proof.
     tauto.
 Qed.
 
-Lemma sound_boxp_absorb_stable {L: Language} {nL: NormalLanguage L} {pL: PropositionalLanguage L} {mL: ModalLanguage L} {MD: Model} {kMD: KripkeModel MD} {M: Kmodel} {R1: KI.Relation (Kworlds M)} {R2: KM.Relation (Kworlds M)} {R3: SS.Relation (Kworlds M)} {R2_incl: Inclusion KM.Krelation SS.Krelation} {SM: Semantics L MD} {kiSM: KripkeIntuitionisticSemantics L MD M SM} {fmSM: FlatModalSemantics L MD M SM} {stableSM: SemanticStable L MD M SM}:
+Lemma sound_boxp_absorb_stable {L: Language} {nL: NormalLanguage L} {pL: PropositionalLanguage L} {mL: ModalLanguage L} {MD: Model} {kMD: KripkeModel MD} {M: Kmodel} {R1: KI.Relation (Kworlds M)} {R2: KM.Relation (Kworlds M)} {R3: SS.Relation (Kworlds M)} {R2_incl: Inclusion KM.Krelation SS.Krelation} {SM: Semantics L MD} {kiSM: KripkeIntuitionisticSemantics L MD M SM} {kpSM: KripkePropositionalSemantics L MD M SM} {fmSM: FlatModalSemantics L MD M SM} {stableSM: SemanticStable L MD M SM}:
   forall x: expr,
     semantic_stable x ->
     (forall (m: Kworlds M), KRIPKE: M, m |= x --> boxp x).
@@ -363,7 +363,7 @@ Proof.
     tauto.
 Qed.
 
-Lemma sound_stable_andp_sepcon1 {L: Language} {nL: NormalLanguage L} {pL: PropositionalLanguage L} {sL: SeparationLanguage L} {MD: Model} {kMD: KripkeModel MD} {M: Kmodel} {R1: KI.Relation (Kworlds M)} {R2: SS.Relation (Kworlds M)} {J: Join (Kworlds M)} {SAabs: SeparationAlgebraAbsorbStable (Kworlds M)} {SM: Semantics L MD} {kiSM: KripkeIntuitionisticSemantics L MD M SM} {fsSM: SeparatingSemantics L MD M SM} {stableSM: SemanticStable L MD M SM}:
+Lemma sound_stable_andp_sepcon1 {L: Language} {nL: NormalLanguage L} {pL: PropositionalLanguage L} {sL: SeparationLanguage L} {MD: Model} {kMD: KripkeModel MD} {M: Kmodel} {R1: KI.Relation (Kworlds M)} {R2: SS.Relation (Kworlds M)} {J: Join (Kworlds M)} {SAabs: SeparationAlgebraAbsorbStable (Kworlds M)} {SM: Semantics L MD} {kiSM: KripkeIntuitionisticSemantics L MD M SM} {kpSM: KripkePropositionalSemantics L MD M SM} {fsSM: SeparatingSemantics L MD M SM} {stableSM: SemanticStable L MD M SM}:
   forall x y z, semantic_stable x ->
     forall m: Kworlds M, KRIPKE: M, m |= (x && y) * z <--> x && (y * z).
 Proof.
