HoareLogic/Sound_Imp.v
@@ -32,7 +32,7 @@ Context {P: ProgrammingLanguage}
         {BSS: BigStepSemantics P model}
         {iBSS: ImpBigStepSemantics P model BSS}.
 
-Context {L: Language} {nL: NormalLanguage L} {pL: PropositionalLanguage L} {SL: SeparationLanguage L} {SM: Semantics L MD} {kiSM: KripkeIntuitionisticSemantics L MD tt SM}.
+Context {L: Language} {nL: NormalLanguage L} {pL: PropositionalLanguage L} {SL: SeparationLanguage L} {SM: Semantics L MD} {kiSM: KripkeIntuitionisticSemantics L MD tt SM} {kpSM: KripkePropositionalSemantics L MD tt SM}.
 
 Lemma hoare_seq_partial_sound: forall c1 c2 P1 P2 P3,
   triple_partial_valid P1 c1 P2 ->
@@ -151,7 +151,7 @@ Context {P: ProgrammingLanguage}
         {BSS: BigStepSemantics P model}
         {iBSS: ImpBigStepSemantics P model BSS}.
 
-Context {L: Language} {nL: NormalLanguage L} {pL: PropositionalLanguage L} {SL: SeparationLanguage L} {SM: Semantics L MD} {kiSM: KripkeIntuitionisticSemantics L MD tt SM}.
+Context {L: Language} {nL: NormalLanguage L} {pL: PropositionalLanguage L} {SL: SeparationLanguage L} {SM: Semantics L MD} {kiSM: KripkeIntuitionisticSemantics L MD tt SM} {kpSM: KripkePropositionalSemantics L MD tt SM}.
 
 
 Lemma hoare_seq_total_sound: forall c1 c2 P1 P2 P3,
