PropositionalLogic/DeepEmbedded/Soundness.v
@@ -19,9 +19,11 @@ Require Logic.PropositionalLogic.DeepEmbedded.KripkeSemantics.
 Local Open Scope logic_base.
 Local Open Scope syntax.
 Local Open Scope kripke_model.
+Local Open Scope kripke_model_class.
 Import PropositionalLanguageNotation.
 Import KripkeModelFamilyNotation.
 Import KripkeModelNotation_Intuitionistic.
+Import KripkeModelClass.
 
 Section Sound.
 
@@ -40,9 +42,8 @@ Instance Trivial_SM: Semantics L Trivial_MD := TrivialSemantics.SM Var.
 Instance Kripke_MD: Model := KripkeSemantics.MD Var.
 Instance Kripke_kMD: KripkeModel Kripke_MD := KripkeSemantics.kMD Var.
 Instance Kripke_R (M: Kmodel): Relation (Kworlds M) := KripkeSemantics.R Var M.
-Instance po_Kripke_R (M: Kmodel): PreOrder (@KI.Krelation _ (Kripke_R M)) := KripkeSemantics.po_R Var M.
 Instance Kripke_SM: Semantics L Kripke_MD := KripkeSemantics.SM Var.
-Instance Kripke_kiSM (M: Kmodel): KripkeIntuitionisticSemantics L Kripke_MD M Kripke_SM := KripkeSemantics.kiSM Var M.
+Instance Kripke_kpSM (M: Kmodel): KripkePropositionalSemantics L Kripke_MD M Kripke_SM := KripkeSemantics.kpSM Var M.
 
 Section Sound_Classical_Trivial.
 
@@ -73,13 +74,16 @@ End Sound_Classical_Trivial.
 Section Sound_Kripke.
 
 Import Logic.PropositionalLogic.Sound.Sound_Kripke.
+Import Logic.PropositionalLogic.DeepEmbedded.KripkeSemantics.
 
-Theorem sound_intuitionistic_Kripke_all: sound Intuitionistic_G Kripke_SM (AllModel _).
+Theorem sound_intuitionistic_Kripke_all:
+  sound Intuitionistic_G Kripke_SM (KripkeModelClass _ (Kmodel_Monotonic + Kmodel_PreOrder)).
 Proof.
   hnf; intros.
-  intros m _.
-  destruct m as [M m].
-  change Kmodel in M.
+  intros _ [M m [mono po_R]].
+  pose proof (@KripkeSemantics.kiSM Var M mono po_R) as kiSM.
+  hnf in mono, po_R.
+  change (Kmodel Var) in M.
   change (Kworlds M) in m.
   change (KRIPKE: M, m |= x).
   induction H.
@@ -96,13 +100,14 @@ Proof.
   + apply sound_falsep_elim.
 Qed.
 
-Theorem sound_weak_classical_Kripke_branch_join: sound DeMorgan_G Kripke_SM (KripkeModelClass _ (KripkeSemantics.Kmodel_BranchJoin Var)).
+Theorem sound_DeMorgan_Kripke_branch_join:
+  sound DeMorgan_G Kripke_SM (KripkeModelClass _
+    (Kmodel_Monotonic + Kmodel_PreOrder + Kmodel_BranchJoin)).
 Proof.
   hnf; intros.
-  intros m ?.
-  destruct H0.
-  unfold KripkeSemantics.Kmodel_BranchJoin in H0.
-  rename H0 into bkiM.
+  intros _ [M m [[mono po_R] bkiM]].
+  pose proof (@KripkeSemantics.kiSM Var M mono po_R) as kiSM.
+  hnf in mono, po_R, bkiM.
   induction H.
   + pose proof sound_modus_ponens x y m.
     exact (H1 IHprovable1 IHprovable2).
@@ -118,13 +123,14 @@ Proof.
   + apply sound_weak_excluded_middle_branch_join.
 Qed.
 
-Theorem sound_GodelDummett_Kripke_no_branch: sound GodelDummett_G Kripke_SM (KripkeModelClass _ (KripkeSemantics.Kmodel_NoBranch Var)).
+Theorem sound_GodelDummett_Kripke_no_branch:
+  sound GodelDummett_G Kripke_SM (KripkeModelClass _
+    (Kmodel_Monotonic + Kmodel_PreOrder + Kmodel_NoBranch)).
 Proof.
   hnf; intros.
-  intros m ?.
-  destruct H0.
-  unfold KripkeSemantics.Kmodel_NoBranch in H0.
-  rename H0 into nkiM.
+  intros _ [M m [[mono po_R] nkiM]].
+  pose proof (@KripkeSemantics.kiSM Var M mono po_R) as kiSM.
+  hnf in mono, po_R, nkiM.
   induction H.
   + pose proof sound_modus_ponens x y m.
     exact (H1 IHprovable1 IHprovable2).
@@ -140,13 +146,14 @@ Proof.
   + apply sound_impp_choice_no_branch.
 Qed.
 
-Theorem sound_classical_Kripke_identity: sound Classical_G Kripke_SM (KripkeModelClass _ (KripkeSemantics.Kmodel_Identity Var)).
+Theorem sound_classical_Kripke_identity:
+  sound Classical_G Kripke_SM (KripkeModelClass _
+    (Kmodel_Monotonic + Kmodel_PreOrder + Kmodel_Identity)).
 Proof.
   hnf; intros.
-  intros m ?.
-  destruct H0.
-  unfold KripkeSemantics.Kmodel_Identity in H0.
-  rename H0 into ikiM.
+  intros _ [M m [[mono po_R] ikiM]].
+  pose proof (@KripkeSemantics.kiSM Var M mono po_R) as kiSM.
+  hnf in mono, po_R, ikiM.
   induction H.
   + pose proof sound_modus_ponens x y m.
     exact (H1 IHprovable1 IHprovable2).
